@prefix ad4gd-procedure: <https://w3id.org/ad4gd/procedures/> .
@prefix ad4gd-prop: <https://w3id.org/ad4gd/properties/> .
@prefix dct: <http://purl.org/dc/terms/> .
@prefix manuf: <https://w3id.org/ad4gd/sensor-manufacturers/> .
@prefix ns1: <http://www.opengis.net/def/metamodel/ogc-na/> .
@prefix owl: <http://www.w3.org/2002/07/owl#> .
@prefix prov: <http://www.w3.org/ns/prov#> .
@prefix qb: <http://purl.org/linked-data/cube#> .
@prefix qudt: <http://qudt.org/schema/qudt/> .
@prefix rdfs: <http://www.w3.org/2000/01/rdf-schema#> .
@prefix schema: <https://schema.org/> .
@prefix skos: <http://www.w3.org/2004/02/skos/core#> .
@prefix sosa: <http://www.w3.org/ns/sosa/> .
@prefix ssn: <http://www.w3.org/ns/ssn/> .
@prefix unit: <http://qudt.org/vocab/unit/> .
@prefix xsd: <http://www.w3.org/2001/XMLSchema#> .

<https://raw.githubusercontent.com/opengeospatial/NamingAuthority/master/generic/entailed/sensors.ttl> a prov:Entity ;
    dct:format "text/turtle" ;
    dct:hasVersion "git:11f77da26d7afa467ccb7490b31e7f2a5c1b7e7a" ;
    prov:wasAttributedTo _:N899146fcf49942b8a6e08ab1bee1d214 ;
    prov:wasGeneratedBy [ a prov:Activity ;
            rdfs:label "Entailment and validation" ;
            rdfs:comment "python ogc.na.update_vocabs -w . .ogc/catalog.ttl --use-git-status --update --graph-store https://defs-dev.opengis.net/fuseki-hosted/data" ;
            prov:endedAtTime "2024-08-12T11:13:16.544621"^^xsd:dateTime ;
            prov:startedAtTime "2024-08-12T11:13:16.124091"^^xsd:dateTime ;
            prov:used [ a prov:Entity ;
                    rdfs:seeAlso <http://defs-dev.opengis.net/ogc-na/scripts/ogc_skos_profile_entailments.ttl> ],
                [ a prov:Entity ;
                    dct:format "text/turtle" ;
                    dct:hasVersion "git:11f77da26d7afa467ccb7490b31e7f2a5c1b7e7a" ;
                    rdfs:seeAlso <https://raw.githubusercontent.com/opengeospatial/NamingAuthority/master/.ogc/catalog.ttl> ],
                [ a prov:Entity ;
                    rdfs:seeAlso <http://defs-dev.opengis.net/ogc-na/definitions/profiles/resources/skos_shared_shacl.ttl> ],
                [ a prov:Entity ;
                    rdfs:seeAlso <http://defs-dev.opengis.net/ogc-na/scripts/ogc_skos_profile.shapes.ttl> ],
                [ a prov:Entity ;
                    rdfs:seeAlso <http://defs-dev.opengis.net/def/metamodel/profiles/skos_shared?_profile=shacl&_mediatype=text/turtle> ],
                [ a prov:Entity ;
                    dct:format "text/turtle" ;
                    dct:hasVersion "git:11f77da26d7afa467ccb7490b31e7f2a5c1b7e7a" ;
                    rdfs:seeAlso <https://raw.githubusercontent.com/opengeospatial/NamingAuthority/master/generic/sensors.ttl> ],
                [ a prov:Entity ;
                    rdfs:seeAlso <http://defs-dev.opengis.net/ogc-na/scripts/skosbasics.shapes.ttl> ],
                [ a prov:Entity ;
                    rdfs:seeAlso <https://datashapes.org/dash.ttl> ],
                [ a prov:Entity ;
                    rdfs:seeAlso <http://www.opengis.net/def/metamodel/profiles/skos_shared> ] ;
            prov:wasAssociatedWith _:N899146fcf49942b8a6e08ab1bee1d214 ;
            prov:wasInformedBy [ dct:identifier "000b0b0e-bf79-4982-95a8-c28d477b078e" ] ] .

<https://w3id.org/ad4gd/air-quality/sensors/> a skos:Collection ;
    dct:provenance "Generated by the OGC Definitions Server to support integration of the elements of this ConceptScheme into bigger collections. ogc_skos_profile_entailements.ttl" ;
    skos:definition "Collection hierarchy for this ConceptScheme" ;
    skos:inScheme <https://w3id.org/ad4gd/air-quality/sensors> ;
    skos:prefLabel "Concepts in AD4GD air quality sensors" .

<https://w3id.org/ad4gd/air-quality/sensors/DHT22> a owl:Class,
        skos:Concept ;
    dct:description """The DHT22 is a basic, low-cost digital temperature and humidity sensor. It uses a capacitive humidity sensor and a thermistor to measure
the surrounding air and spits out a digital signal on the data pin (no analog input pins needed). It's fairly simple to use but requires
careful timing to grab data. The only real downside of this sensor is you can only get new data from it once every 2 seconds, so when using
our library, sensor readings can be up to 2 seconds old.

Low cost
Good for 0-100% humidity readings with 2-5% accuracy
Good for -40 to 80°C temperature readings ±0.5°C accuracy
No more than 0.5 Hz sampling rate (once every 2 seconds)

From: https://www.adafruit.com/product/385
""" ;
    ns1:status <http://www.opengis.net/def/status/valid> ;
    rdfs:subClassOf sosa:Sensor ;
    skos:inScheme <https://w3id.org/ad4gd/air-quality/sensors> ;
    skos:prefLabel "DHT22" ;
    skos:topConceptOf <https://w3id.org/ad4gd/air-quality/sensors> ;
    sosa:observes ad4gd-prop:humidity,
        ad4gd-prop:temperature .

<https://w3id.org/ad4gd/air-quality/sensors/SDS011> a owl:Class,
        skos:Concept ;
    dct:description """This is the specification for the SDS011. One should not consider all those values for granted as there is quite often a big difference
 between what is said to be possible and what is actually possible (and this is why we are setting up all our experiments).

  Output: PM2.5, PM10
  Measuring Range: 0.0-999.9μg/m3
  Response Time 1 second
  Serial Data Output Frequency: 1 time/second
  Particle Diameter Resolution: ≤0.3μm
  Relative Error:10%
  Temperature Range:-20~50°C

Note that the SDS011 humidity working range is 0-70%. Above 70% humidity the readings become unreliable.

From: https://aqicn.org/sensor/sds011/
""" ;
    ns1:status <http://www.opengis.net/def/status/valid> ;
    rdfs:seeAlso <https://aqicn.org/sensor/sds011/> ;
    rdfs:subClassOf sosa:Sensor ;
    skos:inScheme <https://w3id.org/ad4gd/air-quality/sensors> ;
    skos:prefLabel "SDS011" ;
    skos:topConceptOf <https://w3id.org/ad4gd/air-quality/sensors> ;
    sosa:observes [ qudt:hasUnit unit:MicroGM-PER-M3 ;
            skos:broader ad4gd-prop:pm10 ;
            ssn:implements [ qb:order 1 ;
                    skos:broader ad4gd-procedure:pm-humidity-correction ] ],
        ad4gd-prop:pm2.5 ;
    schema:manufacturer manuf:nova-fitness .

<https://w3id.org/ad4gd/air-quality/sensors> a skos:ConceptScheme ;
    dct:source <https://ad4gd.eu/> ;
    ns1:collectionView <https://w3id.org/ad4gd/air-quality/sensors/> ;
    skos:hasTopConcept <https://w3id.org/ad4gd/air-quality/sensors/DHT22>,
        <https://w3id.org/ad4gd/air-quality/sensors/SDS011> ;
    skos:prefLabel "AD4GD air quality sensors" .

[] a prov:Activity ;
    prov:endedAtTime "2024-08-12T11:13:07.667518"^^xsd:dateTime ;
    prov:startedAtTime "2024-08-12T11:13:07.613830"^^xsd:dateTime ;
    prov:used [ a prov:Entity ;
            dct:format "application/json" ;
            dct:hasVersion "git:11f77da26d7afa467ccb7490b31e7f2a5c1b7e7a" ;
            rdfs:seeAlso <file:///home/runner/work/pilot-3-air-quality/pilot-3-air-quality/generic/sensors.yml> ] ;
    prov:wasAssociatedWith [ a prov:Agent,
                schema:SoftwareApplication ;
            rdfs:label "OGC-NA tools" ;
            dct:hasVersion "0.3.50" ;
            rdfs:seeAlso <https://github.com/opengeospatial/ogc-na-tools> ] ;
    prov:wasInformedBy [ dct:identifier "eceaa9a7-e4fe-4a1a-b807-94cb99264b17" ] .

_:N899146fcf49942b8a6e08ab1bee1d214 a prov:Agent,
        schema:SoftwareApplication ;
    rdfs:label "OGC-NA tools" ;
    dct:hasVersion "0.3.50" ;
    rdfs:comment "ogc.na.update_vocabs version 0.3.50" ;
    rdfs:seeAlso <https://github.com/opengeospatial/ogc-na-tools> .

